Bind rule for new typing

src/Functional.v
@@ -1,6 +1,7 @@
 From Heapster Require Import
      Permissions
-     Config.
+     Config
+     NoEvent.
      (* StepError. *)
      (* Typing. *)
 
@@ -19,6 +20,25 @@ From ITree Require Import
 From Paco Require Import
      paco.
 
+Import ITreeNotations.
+
+Ltac rewritebisim lem := pose proof lem as bisim;
+                         eapply bisimulation_is_eq in bisim;
+                         rewrite bisim;
+                         clear bisim.
+
+Ltac rewritebisim_in lem H := pose proof lem as bisim;
+                              eapply bisimulation_is_eq in bisim;
+                              rewrite bisim in H;
+                              clear bisim.
+
+Lemma throw_bind {E R1 R2} `{exceptE unit -< E} (k : R1 -> itree E R2) :
+  x <- throw tt;; k x = throw tt.
+Proof.
+  apply bisimulation_is_eq. pcofix CIH.
+  pstep. unfold throw. rewritebisim @bind_vis. constructor. intros. inversion v.
+Qed.
+
 Section bisim.
   Variant ModifyE {C : Type} : Type -> Type :=
   | Modify : forall (f : C -> C), ModifyE C
@@ -28,65 +48,227 @@ Section bisim.
 
   Context {config specConfig : Type}.
 
-  (* todo move somewhere else *)
+  (* TODO: move somewhere else *)
   Definition sep_step (p q : @perm config specConfig) : Prop :=
     forall r, p ⊥ r -> q ⊥ r.
 
   Inductive typing_gen {R1 R2 : Type} typing (p : perm) (Q : R1 -> R2 -> Perms) :
     itree (E config) R1 -> config -> itree (E specConfig) R2 -> specConfig -> Prop :=
-  | typing_ret r1 c1 r2 c2 :
+  | typing_gen_ret r1 c1 r2 c2 :
       pre p c1 c2 ->
       p ∈ Q r1 r2 ->
       typing_gen typing p Q (Ret r1) c1 (Ret r2) c2
-  | typing_err t1 c1 c2 :
+  | typing_gen_err t1 c1 c2 :
       typing_gen typing p Q t1 c1 (throw tt) c2
-  | typing_tau_L t1 c1 t2 c2 :
+  | typing_gen_tau_L t1 c1 t2 c2 :
       pre p c1 c2 ->
       typing_gen typing p Q t1 c1 t2 c2 ->
       typing_gen typing p Q (Tau t1) c1 t2 c2
-  | typing_tau_R t1 c1 t2 c2 :
+  | typing_gen_tau_R t1 c1 t2 c2 :
       pre p c1 c2 ->
       typing_gen typing p Q t1 c1 t2 c2 ->
       typing_gen typing p Q t1 c1 (Tau t2) c2
-  | typing_tau t1 c1 t2 c2 :
+  | typing_gen_tau t1 c1 t2 c2 :
       pre p c1 c2 ->
       typing p Q t1 c1 t2 c2 ->
       typing_gen typing p Q (Tau t1) c1 (Tau t2) c2
-  | typing_modify_L f k c1 t2 c2 p' :
+  | typing_gen_modify_L f k c1 t2 c2 p' :
       pre p c1 c2 ->
       guar p c1 (f c1) ->
       sep_step p p' ->
       typing_gen typing p' Q (k c1) (f c1) t2 c2 ->
       typing_gen typing p Q (vis (Modify f) k) c1 t2 c2
-  | typing_modify_R t1 c1 f k c2 p' :
+  | typing_gen_modify_R t1 c1 f k c2 p' :
       pre p c1 c2 ->
       sep_step p p' ->
-      typing_gen typing p Q t1 c1 (k c2) (f c2) ->
+      typing_gen typing p' Q t1 c1 (k c2) (f c2) ->
       typing_gen typing p Q t1 c1 (vis (Modify f) k) c2
-  | typing_modify f1 k1 c1 f2 k2 c2 p' :
+  | typing_gen_modify f1 k1 c1 f2 k2 c2 p' :
       pre p c1 c2 ->
       guar p c1 (f1 c1) ->
       sep_step p p' ->
-      typing p Q (k1 c1) (f1 c1) (k2 c2) (f2 c2) ->
+      typing p' Q (k1 c1) (f1 c1) (k2 c2) (f2 c2) ->
       typing_gen typing p Q (vis (Modify f1) k1) c1 (vis (Modify f2) k2) c2
-  | typing_choice_L k c1 t2 c2 p' :
+  | typing_gen_choice_L k c1 t2 c2 p' :
       pre p c1 c2 ->
       sep_step p p' ->
-      (forall b, typing_gen typing p Q (k b) c1 t2 c2) ->
+      (forall b, typing_gen typing p' Q (k b) c1 t2 c2) ->
       typing_gen typing p Q (vis Or k) c1 t2 c2
-  | typing_choice_R t1 c1 k c2 p' :
+  | typing_gen_choice_R t1 c1 k c2 p' :
       pre p c1 c2 ->
       sep_step p p' ->
-      (forall b, typing_gen typing p Q t1 c1 (k b) c2) ->
+      (forall b, typing_gen typing p' Q t1 c1 (k b) c2) ->
       typing_gen typing p Q t1 c1 (vis Or k) c2
-  | typing_choice k1 c1 k2 c2 p' :
+  | typing_gen_choice k1 c1 k2 c2 p' :
       pre p c1 c2 ->
       sep_step p p' ->
-      (forall b1 b2, typing p Q (k1 b1) c1 (k2 b2) c2) ->
+      (forall b1 b2, typing p' Q (k1 b1) c1 (k2 b2) c2) ->
       typing_gen typing p Q (vis Or k1) c1 (vis Or k2) c2
   .
 
-  Definition typing {R1 R2} := paco6 (@typing_gen R1 R2) bot6.
+  Lemma typing_gen_mon {R1 R2} : monotone6 (@typing_gen R1 R2).
+  Proof.
+    repeat intro. induction IN; subst; try solve [econstructor; eauto]; auto.
+  Qed.
+  Hint Resolve typing_gen_mon : paco.
+
+  Definition typing_ {R1 R2} := paco6 (@typing_gen R1 R2) bot6.
+
+  Lemma test {R1 R2} r p Q t c1 s c2 :
+    pre p c1 c2 ->
+    paco6 (@typing_gen R1 R2) r p Q t c1 s c2 ->
+    paco6 (@typing_gen R1 R2) r p Q (Tau t) c1 s c2.
+  Proof.
+    intros. punfold H0. pstep. constructor; auto.
+  Qed.
+
+  Lemma typing_gen_pre {R1 R2} r p (Q : R1 -> R2 -> Perms) t s c1 c2 :
+    typing_gen r p Q t c1 s c2 ->
+    s = throw tt \/ pre p c1 c2.
+  Proof.
+    inversion 1; auto.
+  Qed.
+
+  Definition typing {R1 R2} P Q (t : itree (E config) R1) (s : itree (E specConfig) R2) :=
+    forall p c1 c2, p ∈ P -> pre p c1 c2 -> typing_ p Q t c1 s c2.
+
+  Lemma typing_lte' {R1 R2} p Q Q' (t : itree (E config) R1) (s : itree (E specConfig) R2) c1 c2 :
+    typing_ p Q t c1 s c2 -> (forall r1 r2, Q r1 r2 ⊦ Q' r1 r2) -> typing_ p Q' t c1 s c2.
+  Proof.
+    revert p Q Q' t s c1 c2. pcofix CIH. intros p Q Q' t s c1 c2 Htyping Hlte.
+    punfold Htyping. pstep.
+    induction Htyping; pclearbot; try solve [econstructor; eauto].
+    - constructor; eauto. apply Hlte. auto.
+    - econstructor 11; eauto. right. eapply CIH; eauto. apply H1.
+  Qed.
+
+  Lemma typing_lte {R1 R2} P P' Q Q' (t : itree (E config) R1) (s : itree (E specConfig) R2) :
+    typing P Q t s ->
+    P' ⊦ P ->
+    (forall r1 r2, Q r1 r2 ⊦ Q' r1 r2) ->
+    typing P' Q' t s.
+  Proof.
+    repeat intro.
+    eapply typing_lte'; eauto.
+  Qed.
+
+  Lemma typing_ret {R1 R2} P Q (r1 : R1) (r2 : R2) :
+    P ⊦ Q r1 r2 -> typing P Q (Ret r1) (Ret r2).
+  Proof.
+    repeat intro. pstep. constructor; auto.
+  Qed.
+
+  Lemma rewrite_spin {E R} : (ITree.spin : itree E R) = Tau (ITree.spin).
+  Proof.
+    intros. apply bisimulation_is_eq.
+    ginit. gcofix CIH. gstep. unfold ITree.spin. constructor.
+    apply Reflexive_eqit_gen_eq.
+  Qed.
+
+
+  Lemma typing_spin {R1 R2} P Q :
+    typing P Q (ITree.spin : itree (E config) R1) (ITree.spin : itree (E specConfig) R2).
+  Proof.
+    repeat intro. pcofix CIH. pstep.
+    rewrite (@rewrite_spin _ R1). rewrite (@rewrite_spin _ R2).
+    constructor 5; auto.
+  Qed.
+
+  Lemma typing_top {R1 R2} Q (t : itree (E config) R1) (s : itree (E specConfig) R2) :
+    typing top_Perms Q t s.
+  Proof.
+    repeat intro. inversion H.
+  Qed.
+
+  Lemma typing_bottom' {R1 R2} p Q (t : itree (E config) R1) (s : itree (E specConfig) R2) c1 c2:
+    typing_ p Q t c1 s c2 -> typing_ p (fun _ _ => bottom_Perms) t c1 s c2.
+  Proof.
+    revert p Q t s c1 c2. pcofix CIH. intros. pstep. punfold H0.
+    induction H0; pclearbot; try solve [econstructor; simpl; eauto].
+    econstructor 11; intros; eauto. right. eapply CIH; apply H1.
+  Qed.
+
+  Lemma typing_bottom {R1 R2} P Q (t : itree (E config) R1) (s : itree (E specConfig) R2) :
+    typing P Q t s -> typing P (fun _ _ => bottom_Perms) t s.
+  Proof.
+    repeat intro. eapply typing_bottom'; eauto.
+  Qed.
+
+  Lemma typing_bind' {R1 R2 S1 S2} (p : perm) (Q : R1 -> S1 -> Perms) (R : R2 -> S2 -> Perms)
+        (t1 : itree (E config) R1) (t2 : R1 -> itree (E config) R2)
+        (s1 : itree (E specConfig) S1) (s2 : S1 -> itree (E specConfig) S2)
+        c1 c2 :
+    pre p c1 c2 ->
+    typing_ p Q t1 c1 s1 c2 ->
+    (forall r1 r2, typing (Q r1 r2) R (t2 r1) (s2 r2)) -> (* something to relate r1 and r2? *)
+    typing_ p R (x <- t1 ;; t2 x) c1 (x <- s1 ;; s2 x) c2.
+  Proof.
+    revert p Q R t1 t2 s1 s2 c1 c2. pcofix CIH.
+    intros p Q R t1 t2 s1 s2 c1 c2 Hpre Htyping1 Htyping2.
+    punfold Htyping1. induction Htyping1.
+    - do 2 rewritebisim @bind_ret_l. specialize (Htyping2 _ _ _ c1 c2 H0 H).
+      eapply paco6_mon_bot; eauto.
+    - rewrite throw_bind. pstep. constructor.
+    - rewritebisim @bind_tau.
+      specialize (IHHtyping1 Hpre Htyping2). punfold IHHtyping1.
+      pstep. constructor; auto.
+    - rewritebisim @bind_tau.
+      specialize (IHHtyping1 Hpre Htyping2). punfold IHHtyping1.
+      pstep. constructor; auto.
+    - do 2 rewritebisim @bind_tau. pclearbot.
+      pstep. constructor 5; auto. right. eapply CIH; eauto.
+    - rewritebisim @bind_vis. apply typing_gen_pre in Htyping1. destruct Htyping1; subst.
+      + rewrite throw_bind. pstep. constructor.
+      + specialize (IHHtyping1 H2 Htyping2). punfold IHHtyping1. pstep. econstructor; eauto.
+    - rewritebisim @bind_vis. apply typing_gen_pre in Htyping1. destruct Htyping1; subst.
+      + pstep. econstructor; eauto. rewrite H1. rewrite throw_bind. constructor.
+      + specialize (IHHtyping1 H1 Htyping2). punfold IHHtyping1. pstep. econstructor; eauto.
+    - do 2 rewritebisim @bind_vis. pclearbot.
+      pose proof H2.
+      punfold H2. destruct (typing_gen_pre _ _ _ _ _ _ _ H2).
+      + pstep. econstructor 7; eauto. rewrite H4. rewrite throw_bind. constructor.
+      + pstep. econstructor 8; eauto.
+    - rewritebisim @bind_vis. pstep. econstructor; eauto. intros.
+      destruct (typing_gen_pre _ _ _ _ _ _ _ (H1 b)).
+      + rewrite H3. rewrite throw_bind. constructor.
+      + specialize (H2 b H3 Htyping2). punfold H2.
+    - rewritebisim @bind_vis. pstep. econstructor; eauto. intros.
+      destruct (typing_gen_pre _ _ _ _ _ _ _ (H1 b)).
+      + rewrite H3. rewrite throw_bind. constructor.
+      + specialize (H2 b H3 Htyping2). punfold H2.
+    - do 2 rewritebisim @bind_vis. pclearbot. pstep. econstructor 11; eauto. intros.
+      specialize (H1 b1 b2). punfold H1. destruct (typing_gen_pre _ _ _ _ _ _ _ H1).
+      + left. pstep. rewrite H2. rewrite throw_bind. econstructor; eauto.
+      + right. eapply CIH; eauto. pstep; eauto.
+  Qed.
+
+  Lemma typing_bind {R1 R2 S1 S2} (P : Perms) (Q : R1 -> S1 -> Perms) (R : R2 -> S2 -> Perms)
+        (t1 : itree (E config) R1) (t2 : R1 -> itree (E config) R2)
+        (s1 : itree (E specConfig) S1) (s2 : S1 -> itree (E specConfig) S2) :
+    typing P Q t1 s1 ->
+    (forall r1 r2, typing (Q r1 r2) R (t2 r1) (s2 r2)) -> (* something to relate r1 and r2? *)
+    typing P R (x <- t1 ;; t2 x) (x <- s1 ;; s2 x).
+  Proof.
+    repeat intro.
+    eapply typing_bind'; eauto.
+  Qed.
+
+  (* TODO with a custom definition of no error *)
+  (* Lemma typing_soundness {R1 R2} Q (t : itree (E config) R1) (s : itree (E specConfig) R2) : *)
+  (*       forall p c1 c2, typing_ p Q t c1 s c2 -> *)
+  (*                  no_event_l s -> *)
+  (*                  no_event_l t. *)
+  (* Proof. *)
+  (*   revert Q t s. pcofix CIH. intros Q t s p c1 c2 Htyping Hs. pstep. *)
+  (*   punfold Htyping. pinversion Hs. *)
+  (*   - (* rewrite (itree_eta_ s) in Htyping. unfold E in Htyping. rewrite <- H0 in Htyping.  *) *)
+  (*     clear H0. *)
+  (*     induction Htyping; intros; try solve [constructor; auto]. *)
+  (*     + (* throw *) inversion Hs. *)
+  (*     + (* TauR *) inversion Hs. pclearbot. pinversion H1; eauto. *)
+  (*     + (* Tau *) inversion Hs. pclearbot. constructor. right. eapply CIH; eauto. *)
+  (*     + (* ModifyL *) constructor; intros. left. pstep. apply IHHtyping. *)
+  (* Qed. *)
 
 End bisim.
 
